pre unfold addition

lemma/live_proc.v
@@ -51,13 +51,45 @@ Proof.
     eapply pc_trans with (M':= (p <-- y));try easy.
     eapply pc_subm. easy.
 Qed.
-
+(*
 Hint Resolve betaPr_unfold_one :procs.
 
+Fixpoint is_unfolded Q := 
+    match Q with 
+    | p_inact => True
+    | p_send _ _ _ _ => True
+    | p_recv _ _ => True
+    | p_ite e p1 p2 => is_unfolded p1 /\ is_unfolded p2 
+    | _ => False end.
+
+
+Lemma guardP_break_plus : forall P, all_guarded P -> exists Q, 
+    forall r, unfoldP (r <-- P) (r <-- Q) /\ is_unfolded Q.
+Proof.
+    intros.
+    induction P;
+    eapply guardP_break in H as Hguard; destr_hyps;
+    try solve [
+    exists x;intros;split;try eauto with procs;inversion H0;subst;easy].
+    eapply guarded_after_multi_unfold in H as Hguard';try exact H0.
+    
+    destruct H1 as [Hu | [Hu | [Hu | Hu]]];destr_hyps;subst;
+    inversion H0;subst;try easy.
+    eapply guard_ite_inv in Hguard'. destr_hyps.
+    specialize (IHP1 H1). specialize (IHP2 H2).
+    destr_hyps.
+    exists (p_ite x0 x3 x2). intros. specialize (H4 r). specialize (H3 r).
+    destr_hyps.
+    split;try eauto with procs.
+    Search unfoldP.
+    inversion H0;subst. clear H1.
+*)
+
+(*
 Lemma inv_proc_send : forall M gamma p q xsp, typ_sess M gamma ->
-M.find p gamma = Some (ltt_send q xsp) -> exists M' M'' P' e ell,
-betaRtc M M' /\ 
-unfoldP M' ((p <-- p_send q ell e P')||| M'').
+M.find p gamma = Some (ltt_send q xsp) -> (exists M' M'' P' e ell,
+(betaRtc M M' \/ unfoldP M M') /\ 
+unfoldP M' ((p <-- p_send q ell e P')||| M'')).
 Proof.
     intros * Hsess Hfindp.
     assert(Hinp:InT p M) by (
@@ -77,20 +109,49 @@ Proof.
             rewrite Hfindp in H2;inversion H2;subst;clear H2. tauto.
         }
         destruct Hprocs as [Hproc Hguard].
-        eapply guardP_break in Hguard as Htr;destr_hyps. rename H into Punf.
-        eapply typ_proc_after_betaPr in Punf as Htyp';try exact Hproc.
-        rename H0 into Htr.
+        evar (Cs: list (option sort)).
+        evar (Ct: list (option ltt)).
+        instantiate (Ct:=[]).
+        instantiate (Cs:=[]).
         generalize dependent M.
-        pose proof Htyp' as Htyp.
-        generalize dependent P. 
+        generalize dependent M'.
+        generalize dependent gamma.
+        fold Cs in Hproc.
+        fold Ct in Hproc.
+        clearbody Cs Ct.
+        pose proof Hproc as Htyp'.
         dependent induction Htyp'.
         {
-            intros.
-            destruct Htr as [Hu | [Hu | [Hu | Hu]]];destr_hyps;subst;easy. 
+            specialize (Hguard 1). destr_hyps. inversion H1. 
         }
         {
             intros.
-            destruct Htr as [Hu | [Hu | [Hu | Hu]]];destr_hyps;subst;easy. 
+            assert(exists Q, substitutionP 0 0 0 (p_rec p0) p0 Q).
+            {
+                eapply guardP_break in Hguard.
+                destr_hyps. inversion H;subst.
+                destruct H0 as [H0 | [H0 | [H0 | H0]]];destr_hyps;subst; try easy.
+                inversion H1;subst.
+                exists y;easy.
+            }
+            destruct H as [Q Hsubst].
+            Search substitutionP typ_proc.
+            eapply IHHtyp' with (,:=in Htyp'.
+            eapply inv_proc_rec in Hproc;try reflexivity. destr_hyps.
+            eapply subst_proc_varf in Hsubst;try exact H.
+            Print typ_proc.
+ 
+            
+            assert(typ_proc cs (Some (ltt_send q xsp) :: ct) p0 (ltt_send q xsp)) by admit.
+
+            eapply IHHtyp' in H1;try easy.
+            intros.
+            specialize (Hguard n). destr_hyps. inversion H2;subst. exists 0. constructor.
+            Search guardP substitutionP.
+            assert(betaPr (p_rec p0) Q). constructor;easy.
+            Search guardP betaPr.
+            eapply gp_rec in H4;try exact H7. Print guardP.
+            inversion Hproc;subst.
         }
         {
             intros. eapply inv_proc_ite in Htyp;try reflexivity;destr_hyps.
@@ -111,8 +172,7 @@ Proof.
                 destr_hyps.   
                 eauto with procs.
             }
-            eapply expr_eval_b in H4. destruct H4.
-            
+            eapply expr_eval_b in H4. destruct H4.            
 
             assert(Hbet: betaP ((p <-- p_ite e p1 p2) ||| M') ((p <-- p1) ||| M'))
             by (eapply rt_ite;easy).
@@ -123,12 +183,165 @@ Proof.
         induction Punf.
         assert(typ_proc [] [] )
     }
-Theorem sess_fidelity : forall M gamma p q ell gamma', 
-typ_sess M gamma -> tctxR gamma (lcomm p q ell) gamma' ->
-    exists gamma'' M', tctxR gamma (lcomm p q ell) gamma'' /\ betaRtc M M' /\ typ_sess M' gamma''.
+*)
+
+
+Lemma typ_proc_inv_send : forall M gamma p q xsp xsq, typ_sess M gamma ->
+    M.find p gamma = Some (ltt_send q xsp) ->
+    M.find q gamma = Some (ltt_recv p xsq) ->
+    (exists Mr ell e P', unfoldP M ((p <-- p_send q ell e P') ||| Mr)) \/
+    (exists Mr e Pt Pf, unfoldP M ((p <-- p_ite e Pt Pf) ||| Mr)).
+Proof.
+    intros * Hsess Hfindp Hfindq.
+    assert(Hpq: p <> q) by (red;intros;subst;congruence).
+    eapply canonical_glob_nt with (xsq:=xsq) in Hfindp as Hcanon;try exact Hsess;try easy.
+    destruct Hcanon.
+    {
+        destr_hyps. eapply typ_after_unfold in H as Htu;try exact Hsess. inversion Htu;subst.
+        inversion_clear H3. inversion_clear H4. inversion_clear H3 . inversion_clear H6.
+        destr_hyps.
+        assert(x3=ltt_send q xsp) by (congruence);subst.
+        assert(x2=ltt_recv p xsq) by congruence;subst.
+        eapply guardP_break in H10;destr_hyps.
+        destruct H12 as [Hdr | [Hdr | [Hdr |Hdr]]];destr_hyps;subst;eapply typ_proc_after_betaPr in H10 as Htunf;try exact H9.
+        {
+         eapply inv_proc_inact in Htunf;easy.
+        }
+        {
+            right.
+            exists ((q <-- x1) ||| x), x3, x5, x6.
+            assert(unfoldP M ((p <-- x0) ||| ((q <-- x1) ||| x))). eauto with procs.
+            assert(multi betaPr x1 x1) by constructor.
+            eauto with procs.
+        }
+        {
+            left. 
+            eapply inv_proc_send in Htunf as Ht;try reflexivity. 
+            destr_hyps. pinversion H14;subst;try apply sub_mon.
+            
+            exists ((q <-- x1) ||| x), x5, x6, x7.
+            assert(multi betaPr x1 x1) by constructor. eauto with procs.
+        }
+        {
+            eapply inv_proc_recv in Htunf;try reflexivity. destr_hyps. pinversion H13;try apply sub_mon.   
+        }
+    }
+    {
+        destr_hyps. eapply typ_after_unfold in H as Htu;try exact Hsess. inversion Htu;subst.
+        inversion_clear H3. inversion_clear H4. inversion_clear H3 . inversion_clear H5.
+        destr_hyps.
+        assert(x1=ltt_send q xsp) by (congruence);subst.
+        assert(x2=ltt_recv p xsq) by congruence;subst.
+        eapply guardP_break in H9;destr_hyps.
+        destruct H11 as [Hdr | [Hdr | [Hdr |Hdr]]];destr_hyps;subst;eapply typ_proc_after_betaPr in H9 as Htunf;try exact H8.
+        {
+         eapply inv_proc_inact in Htunf;easy.
+        }
+        {
+            right.
+            exists ((q <-- x0)), x2, x4, x5.
+            assert(unfoldP M ((p <-- x) ||| ((q <-- x0)))). eauto with procs.
+            assert(multi betaPr x0 x0) by constructor.
+            eauto with procs.
+        }
+        {
+            left. 
+            eapply inv_proc_send in Htunf as Ht;try reflexivity. 
+            destr_hyps. pinversion H13;subst;try apply sub_mon.
+            
+            exists ((q <-- x0) ), x4, x5, x6.
+            assert(multi betaPr x0 x0) by constructor. eauto with procs.
+        }
+        {
+            eapply inv_proc_recv in Htunf;try reflexivity. destr_hyps. pinversion H12;try apply sub_mon.   
+        }
+    }
+Qed.
+
+Lemma SList_extendLis {A:Type}: forall n (a:A), SList (extendLis n (Some a)).
+                Proof.
+                    induction n;intros; simpl;easy.
+                Qed.
+(*
+Theorem sess_fidelity_send : forall M gamma p q   ell gamma', 
+typ_sess M gamma -> tctxR gamma (lcomm p q ell) gamma' -> 
+    (exists gamma'' M' ell', tctxR gamma (lcomm p q ell') gamma'' /\ 
+    betaP M M' /\ typ_sess M' gamma'') \/
+    (exists gamma M', 
+    betaP M M' /\ typ_sess M' gamma).
 Proof.
     intros * Hsess Hstep.
-    inversion Hsess;subst. rename H into Htwf, H0 into Hin, H1 into Hndup, H2 into Hfat.
+    eapply lem_6_11c_tctx_comm_invert in Hstep;destr_hyps.
+    eapply typ_proc_inv_send in H as Hp_dil;try exact Hsess;try exact H0.
+    destruct Hp_dil.
+    {
+        destr_hyps.
+        left.
+        eapply typ_after_unfold in H6 as Hu;try exact Hsess.
+        assert ((exists Q M', unfoldP x5 ((q <-- Q) ||| M')) \/ (exists Q, unfoldP x5 ((q <-- Q)))).
+        {
+            inversion Hu;subst.
+            assert(Hinq : InT q ((p <-- p_send q x6 x7 x8) ||| x5)).
+            {
+                eapply H8;red;exists (ltt_recv p x3);split;easy.   
+            }
+            red in Hinq. simpl in Hinq.
+            destruct Hinq;subst;try congruence. assert(InT q x5) by (red;easy).
+            eapply move_forward_h in H12;destr_hyps.
+            destruct H12. destr_hyps. left. exists x10, x11;easy.
+            right. destr_hyps. exists x10;easy.
+        }
+        destruct H7 as [Hunfq | Hunfq];destr_hyps.
+        {
+            assert (Hunfm :unfoldP M ((p <-- p_send q x6 x7 x8) |||( (q <-- x9) ||| x10))).
+            {
+                eauto with procs.   
+            }
+            eapply typ_after_unfold in Hunfm as Hsess2;try exact Hsess.
+            inversion Hsess2;subst. inversion_clear H11. inversion_clear H13.
+            inversion_clear H11. inversion_clear H12.
+            destr_hyps.
+            assert(x11 = ltt_send q x1) by congruence.
+            assert(x12 = ltt_recv p x3) by congruence.
+            subst.
+            eapply inv_proc_send in H15;try reflexivity. destr_hyps.
+            assert(exists gamma'', tctxR gamma (lcomm p q x6) gamma'').
+            {
+                rename x13 into g.
+                assert (assoc.issubProj (ltt_send q (extendLis x6 (Some (x11, x12)))) g p).
+                {
+                    eapply assoc_inv_find with (g:=g) in H11;try easy.
+                    red in H11. destr_hyps.
+                    red. exists x13. split;try easy. eapply stTrans;try exact H21;easy.
+                }
+                eapply assoc_inv_find with (g:=g) in H12 as Hinf;try easy.
+                assert(SList x3).
+                {
+                    red in H8. specialize (H8 _ _ H12). pinversion H8;subst;try easy;try apply wfltt.wfltt_mon.   
+                }
+                assert (isgPartsC p g).
+                {
+                    red in H22. destr_hyps. destruct (decidable.decidable_isgPartsC g p);try easy.
+                    eapply assoc.subtype_send_inv1 in H24;destr_hyps;subst. pinversion H22;subst;try easy;
+                    try apply proj_mon.   
+                }
+                eapply assoc.lem_6_16_simul_subproj in H22;try exact Hinf;try easy;
+                try eapply SList_extendLis.
+                assert(onth x6 (extendLis x6 (Some (x11, x12)))=Some (x11,x12)) by (rewrite extendExtract;easy).
+                
+                eapply Forall2R_prop in H22;try exact H25;tac_sanitize.
+                eapply simpl
+                Search tctxR M.find.
+                Search "simul" assoc.issubProj.
+            }
+        }
+    }    
+
+    eapply typ_after_unfold in Hunf as Hsess';try exact Hsess.
+    inversion Hsess';subst. 
+    
+    rename H into Htwf, H0 into Hin, H1 into Hndup, H2 into Hfat.
+
     eapply lem_6_11c_tctx_comm_invert in Hstep;destr_hyps.
     assert(Hpq_neq: p <> q) by (red;intros;subst;congruence).
     assert(Hinp: InT p M) by (eapply Hin;red; exists (ltt_send q x2);easy).
@@ -229,6 +442,7 @@ Proof.
         
     }
     specialize (Hin p). unfold in_not_end in Hin.
+*)
 
 Definition live_sess (Mp:session) := forall M p q ell e P' Mr, betaRtc Mp M -> 
     (unfoldP M (p <-- p_send q ell e P' ||| Mr)) -> exists M', betaRtc M M' /\
